Fcomp/Degree.lean
@@ -1,0 +1,30 @@
+/-
+  Degree.lean
+  Definition of the degree of a term.
+-/
+
+import Fcomp.Terms
+import Fcomp.Types
+import Fcomp.Context
+import Fcomp.Beta
+
+namespace Fcomp.STLC
+
+/-! ### Degree of a Term -/
+
+/-- Compute the degree of a term. -/
+@[simp]
+def degree : Term → Nat
+  | Term.var _ => 0
+  | Term.abs _ _ t => (degree t) + 1
+  | Term.app t₁ t₂ => Nat.max (degree t₁) (degree t₂)
+  | Term.pair t₁ t₂ => Nat.max (degree t₁) (degree t₂)
+  | Term.fst t => degree t
+  | Term.snd t => degree t
+  | Term.inl _ t => degree t
+  | Term.inr _ t => degree t
+  | Term.case t _ b₁ _ b₂ => Nat.max (degree t) (Nat.max (degree b₁) (degree b₂))
+  | Term.abort _ t => degree t
+  | Term.unitVal => 0
+
+end Fcomp.STLC
